rules/rules_squiggle2.v
@@ -442,26 +442,35 @@ Qed.
     H, z : T[b], J |- C ext t
     H, z : T[a], J |- a ~ b
 >>
-*)
+ *)
+
+Definition rule_cequiv_subst_hyp_concl {o} (H : @bhyps o) z T x a J C t :=
+  mk_baresequent (snoc H (mk_hyp z (subst T x a)) ++ J) (mk_concl C t).
+
+Definition rule_cequiv_subst_hyp_hyp1 {o} (H : @bhyps o) z T x b J C t :=
+  mk_baresequent (snoc H (mk_hyp z (subst T x b)) ++ J) (mk_concl C t).
+
+Definition rule_cequiv_subst_hyp_hyp2 {o} (H : @bhyps o) z T x a J b e :=
+  mk_baresequent (snoc H (mk_hyp z (subst T x a)) ++ J) (mk_concl (mk_cequiv a b) e).
 
 Definition rule_cequiv_subst_hyp {o}
            (H J : @barehypotheses o)
            (x z : NVar)
-           (C T a b t  : NTerm) :=
+           (C T a b t e : NTerm) :=
   mk_rule
-    (mk_baresequent (snoc H (mk_hyp z (subst T x a)) ++ J) (mk_concl C t))
-    [ mk_baresequent (snoc H (mk_hyp z (subst T x b)) ++ J) (mk_concl C t),
-      mk_baresequent (snoc H (mk_hyp z (subst T x a)) ++ J) (mk_conclax (mk_cequiv a b))
+    (rule_cequiv_subst_hyp_concl H z T x a J C t)
+    [ rule_cequiv_subst_hyp_hyp1 H z T x b J C t,
+      rule_cequiv_subst_hyp_hyp2 H z T x a J b e
     ]
     [].
 
 Lemma rule_cequiv_subst_hyp_true {o} :
   forall lib (H J : @barehypotheses o)
          (x z : NVar)
-         (C T a b t  : NTerm)
+         (C T a b t e : NTerm)
          (bc1 : disjoint (free_vars a) (bound_vars T))
          (bc2 : disjoint (free_vars b) (bound_vars T)),
-    rule_true lib (rule_cequiv_subst_hyp H J x z C T a b t).
+    rule_true lib (rule_cequiv_subst_hyp H J x z C T a b t e).
 Proof.
   intros.
   unfold rule_cequiv_subst_hyp, rule_true, closed_type_baresequent, closed_extract_baresequent; simpl.
@@ -527,427 +536,474 @@ Proof.
   generalize (in_deq NVar deq_nvar x (free_vars T)); introv i.
   destruct i as [i | i].
 
-  (* First, we assume that x is in the free variables of T.
-   * We can now prove that a and b depend on H only. *)
-
-  assert (covered a (vars_hyps H))
-         as cvah
-         by (clear hyp1 hyp2;
-             allapply @vswf_hypotheses_nil_implies;
-             rw @wf_hypotheses_app in wh2; repnd;
-             rw @wf_hypotheses_snoc in wh0; repnd; allsimpl;
-             allrw @isprog_vars_eq; repnd;
-             unfold covered;
-             generalize (eqvars_free_vars_disjoint T [(x,a)]);
-             introv e; rw @fold_subst in e; simpl in e;
-             apply subvars_eqvars with (s2 := vars_hyps H) in e; auto;
-             rw subvars_prop in e;
-             rw subvars_prop; introv j;
-             revert e; boolvar; try (complete sp); simpl; intro e;
-             apply e; rw in_app_iff; rw app_nil_r; sp).
-
-  assert (covered b (vars_hyps H))
-         as cvbh
-         by (clear hyp1 hyp2;
-             allapply @vswf_hypotheses_nil_implies;
-             rw @wf_hypotheses_app in wh1; repnd;
-             rw @wf_hypotheses_snoc in wh0; repnd; allsimpl;
-             allrw @isprog_vars_eq; repnd;
-             unfold covered;
-             generalize (eqvars_free_vars_disjoint T [(x,b)]);
-             introv e; rw @fold_subst in e; simpl in e;
-             apply subvars_eqvars with (s2 := vars_hyps H) in e; auto;
-             rw subvars_prop in e;
-             rw subvars_prop; introv j;
-             revert e; boolvar; try (complete sp); simpl; intro e;
-             apply e; rw in_app_iff; rw app_nil_r; sp).
-
-  assert (covered T (snoc (vars_hyps H) x))
-         as covT
-         by (clear hyp1 hyp2;
-             allapply @vswf_hypotheses_nil_implies;
-             rw @wf_hypotheses_app in wh1; repnd;
-             rw @wf_hypotheses_snoc in wh0; repnd; allsimpl;
-             allrw @isprog_vars_eq; repnd;
-             unfold covered;
-             generalize (eqvars_free_vars_disjoint T [(x,b)]);
-             introv e; rw @fold_subst in e; simpl in e;
-             apply subvars_eqvars with (s2 := vars_hyps H) in e; auto;
-             rw subvars_prop in e;
-             rw subvars_prop; introv j;
-             revert e; boolvar; try (complete sp); simpl; intro e;
-             rw in_snoc;
-             destruct (deq_nvar x0 x); subst; sp;
-             left; apply e; rw in_app_iff; rw app_nil_r; rw in_remove_nvars; rw in_single_iff; sp).
-
-  assert (!LIn z (free_vars a))
-         as niza
-         by (intro j; unfold covered in cvah;
-             rw subvars_prop in cvah; apply cvah in j; sp).
-
-  assert (!LIn z (free_vars b))
-         as nizb
-         by (intro j; unfold covered in cvbh;
-             rw subvars_prop in cvbh; apply cvbh in j; sp).
-
-  assert (disjoint (free_vars a) (vars_hyps J))
-         as daj
-         by (introv j k; unfold covered in cvah;
-             rw subvars_prop in cvah; apply cvah in j; sp;
-             apply disjHJ in j; sp).
-
-  assert (disjoint (free_vars b) (vars_hyps J))
-         as dbj
-         by (introv j k; unfold covered in cvbh;
-             rw subvars_prop in cvbh; apply cvbh in j; sp;
-             apply disjHJ in j; sp).
-
-  assert (subvars (free_vars (subst T x a)) (vars_hyps H))
-         as svaH
-         by (generalize (eqvars_free_vars_disjoint T [(x,a)]); intro e;
-             apply eqvars_sym in e;
-             apply subvars_eqvars with (s2 := vars_hyps H) in e; auto;
-             rw subvars_prop; introv; simpl;
-             rw in_app_iff; rw in_remove_nvars; rw in_single_iff;
-             boolvar; simpl; try (complete sp);
-             rw app_nil_r; intro j; repdors; repnd;
-             try (complete (unfold covered in covT; rw subvars_prop in covT;
-                            apply covT in j1; rw in_snoc in j1; allrw; sp));
-             try (complete (unfold covered in cvah; rw subvars_prop in cvah;
-                            apply cvah in j; sp))).
-
-  assert (subvars (free_vars (subst T x b)) (vars_hyps H))
-         as svbH
-         by (generalize (eqvars_free_vars_disjoint T [(x,b)]); intro e;
-             apply eqvars_sym in e;
-             apply subvars_eqvars with (s2 := vars_hyps H) in e; auto;
-             rw subvars_prop; introv; simpl;
-             rw in_app_iff; rw in_remove_nvars; rw in_single_iff;
-             boolvar; simpl; try (complete sp);
-             rw app_nil_r; intro j; repdors; repnd;
-             try (complete (unfold covered in covT; rw subvars_prop in covT;
-                            apply covT in j1; rw in_snoc in j1; allrw; sp));
-             try (complete (unfold covered in cvbh; rw subvars_prop in cvbh;
-                            apply cvbh in j; sp))).
-
-  assert (subvars (free_vars T) (x :: vars_hyps H))
-         as svTH
-         by (rw subvars_prop in covT; rw subvars_prop; introv j;
-             apply covT in j; rw in_snoc in j; simpl; sp).
-
-  generalize (hyp1 s1 s2); clear hyp1; intro hyp1.
-
-  autodimp hyp1 hyp.
-
-
-  (* First, we prove that the hypotheses of the first sequent are functional *)
-  introv sim'.
-  rw @similarity_app in sim'; simpl in sim'; exrepnd; subst; allrw length_snoc; cpx.
-  rw @similarity_snoc in sim'5; simpl in sim'5; exrepnd; subst; allrw length_snoc; cpx.
-
-  rw @eq_hyps_app.
-  exists (snoc s1a0 (z, t1)) s1b (snoc s2a0 (z, t2)) s2b.
-  allrw length_snoc; dands; try (complete sp).
-
-  assert (cover_vars (subst T x b) s2a0)
-    as cov2
-      by (apply cover_vars_change_sub with (sub1 := s1a0); sp;
-          allapply @similarity_dom; repnd; allrw; sp).
-
-  rw @eq_hyps_snoc; simpl.
-  exists s1a0 s2a0 t1 t2 w p cov2.
-  dands; try (complete sp).
-
-  assert (wf_term (subst T x a))
-    as wfsa
-      by (apply @lsubst_preserves_wf_term; simpl;
-          unfold wf_sub, sub_range_sat; simpl; sp; cpx; rw @nt_wf_eq; sp).
-
-  assert (cover_vars (subst T x a) s1a0)
-    as cova1 by (rw @cover_vars_eq; allapply @similarity_dom; repnd; allrw; sp).
-
-  dup eqh as hf.
-
-  apply hyps_functionality_init_seg
-  with (s3 := s2b) in eqh; auto.
-  apply @hyps_functionality_init_seg_snoc2
-  with (t' := t2) (w := wfsa) (c := cova1) in eqh.
-  apply eqh in sim'6; auto.
-
-  generalize (hyp2 (snoc s1a0 (z,t1) ++ s1b) s2 hf sim); clear hyp2; intro hyp2; exrepnd.
-  lsubst_tac.
-  rw @member_eq in hyp1.
-  rw <- @member_cequiv_iff in hyp1.
-  spcast.
-
-  assert (cover_vars_upto T (csub_filter s1a0 [x]) [x])
-         as covT1
-         by (unfold cover_vars_upto; unfold covered in covT;
-             rw @dom_csub_csub_filter;
-             rw subvars_app_remove_nvars_r; simpl;
-             allapply @similarity_dom; repnd; allrw; sp).
-
-  generalize (simple_lsubstc_subst b x T w s1a0 p wb c6 wT covT1);
-    introv e; autodimp e hyp.
-  rw e in sim'2; clear e.
-
-  generalize (simple_lsubstc_subst a x T wfsa s1a0 cova1 wa c4 wT covT1);
-    introv e; autodimp e hyp.
-  rw e; clear e.
-
-  apply cequivc_preserving_equality
-  with (A := substc (lsubstc b wb s1a0 c6) x
-                    (lsubstc_vars T wT (csub_filter s1a0 [x]) [x] covT1));
-    auto;
-    try (complete (apply cequivc_sym; eauto with cequivc)).
-
-
-  (* now we prove the tequality of T[x\b] *)
-  assert (wf_term (subst T x a))
-         as wfsa
-         by (apply @lsubst_preserves_wf_term; sp;
-             unfold wf_sub, sub_range_sat; simpl; sp; cpx; rw @nt_wf_eq; sp).
-
-  assert (cover_vars (subst T x a) s1a0)
-         as covsa1 by (rw @cover_vars_eq; allapply @similarity_dom; repnd; allrw; sp).
-
-  generalize (eqh (snoc s2a0 (z,t1) ++ s1b)); intro eqhy.
-  autodimp eqhy hyp.
-  rw @similarity_app; simpl.
-  exists (snoc s1a0 (z, t1)) s1b (snoc s2a0 (z, t1)) s1b; allrw length_snoc; sp.
-  rw @similarity_snoc; simpl.
-  exists s1a0 s2a0 t1 t1 wfsa covsa1; sp.
-
-  rw @similarity_app in sim; simpl in sim; exrepnd.
-  apply app_split in sim0; allrw length_snoc; repnd; subst;
-  try (complete (allapply @similarity_dom; repnd; allrw; sp)).
-  rw @similarity_snoc in sim5; simpl in sim5; exrepnd; cpx; proof_irr.
-  apply equality_refl in sim2; sp.
-
-  apply @similarity_refl in sim'1; sp.
-
-  rw @eq_hyps_app in eqhy; simpl in eqhy; exrepnd.
-  apply app_split in eqhy0; allrw length_snoc; repnd; subst; cpx;
-  try (complete (allapply @similarity_dom; repnd; allrw; sp)).
-  apply app_split in eqhy2; allrw length_snoc; repnd; subst; cpx;
-  try (complete (allapply @similarity_dom; repnd; allrw; sp)).
-  rw @eq_hyps_snoc in eqhy5; simpl in eqhy5; exrepnd; cpx.
-
-  (* now we prove the tequality from eqhy0 *)
-
-  generalize (hyp2 (snoc s1a (z,t0) ++ s2b0)
-                   (snoc s2a (z,t0) ++ s2b0)
-                   eqh); clear hyp2; intro hyp2.
-  (* before using hyp2 we have to prove a few things *)
-  autodimp hyp2 hyp.
-  rw @similarity_app; simpl.
-  exists (snoc s1a (z,t0)) s2b0 (snoc s2a (z,t0)) s2b0; allrw length_snoc; sp.
-  rw @similarity_snoc; simpl.
-  exists s1a s2a t0 t0 w0 p1; sp.
-
-  rw @similarity_app in sim; simpl in sim; exrepnd.
-  apply app_split in sim0; allrw length_snoc; repnd; subst;
-  try (complete (allapply @similarity_dom; repnd; allrw; sp)).
-  rw @similarity_snoc in sim5; simpl in sim5; exrepnd; cpx; proof_irr.
-  apply equality_refl in sim2; sp.
-
-  apply @similarity_refl in sim'1; sp.
-  (* now we start using hyp2 *)
-  exrepnd.
-  lsubst_tac.
-  rw @tequality_mkc_cequiv in hyp0.
-  rw @member_eq in hyp1.
-  rw <- @member_cequiv_iff in hyp1.
-  appdup hyp0 hyp1.
-  spcast.
-
-  assert (cover_vars_upto T (csub_filter s1a [x]) [x])
-         as cvuT1
-         by (unfold cover_vars_upto; unfold covered in covT;
-             rw @dom_csub_csub_filter;
-             rw subvars_app_remove_nvars_r; simpl;
-             allapply @similarity_dom; repnd; allrw; sp).
-
-  assert (cover_vars_upto T (csub_filter s2a [x]) [x])
-         as cvuT2
-         by (unfold cover_vars_upto; unfold covered in covT;
-             rw @dom_csub_csub_filter;
-             rw subvars_app_remove_nvars_r; simpl;
-             allapply @similarity_dom; repnd; allrw; sp).
-
-  generalize (simple_lsubstc_subst b x T w s1a p wb c6 wT cvuT1);
-    intro e; autodimp e hyp.
-  rw e; clear e.
-
-  generalize (simple_lsubstc_subst b x T w s2a cov2 wb c10 wT cvuT2);
-    intro e; autodimp e hyp.
-  rw e; clear e.
-
-  generalize (simple_lsubstc_subst a x T w0 s1a p1 wa c4 wT cvuT1);
-    intro e; autodimp e hyp.
-  rw e in eqhy0; clear e.
-
-  generalize (simple_lsubstc_subst a x T w0 s2a p2 wa c8 wT cvuT2);
-    intro e; autodimp e hyp.
-  rw e in eqhy0; clear e.
-
-  apply tequality_respects_cequivc_left
-        with (T1 := substc (lsubstc a wa s1a c4) x
-                           (lsubstc_vars T wT (csub_filter s1a [x]) [x] cvuT1));
-    try (complete (eauto with cequivc)).
-
-  apply tequality_respects_cequivc_right
-  with (T2 := substc (lsubstc a wa s2a c8) x
-                     (lsubstc_vars T wT (csub_filter s2a [x]) [x] cvuT2));
-    auto;
-    try (complete (eauto with cequivc)).
-
-
-  (* Now we prove the sub_eq_hyps *)
-
-  assert (wf_term (subst T x a))
-         as wfsa
-         by (apply @lsubst_preserves_wf_term; sp;
-             unfold wf_sub, sub_range_sat; simpl; sp; cpx; rw @nt_wf_eq; sp).
-
-  assert (cover_vars (subst T x a) s1a0)
-         as covsa1 by (rw @cover_vars_eq; allapply @similarity_dom; repnd; allrw; sp).
-
-  generalize (hyp2 (snoc s1a0 (z,t1) ++ s1b)
-                   (snoc s2a0 (z,t1) ++ s1b)
-                   eqh); clear hyp2; intro hyp2.
-  (* before using hyp2 we have to prove a few things *)
-  autodimp hyp2 hyp.
-  rw @similarity_app; simpl.
-  exists (snoc s1a0 (z,t1)) s1b (snoc s2a0 (z,t1)) s1b; allrw length_snoc; sp.
-  rw @similarity_snoc; simpl.
-  exists s1a0 s2a0 t1 t1 wfsa covsa1; sp.
-
-  rw @similarity_app in sim; simpl in sim; exrepnd.
-  apply app_split in sim0; allrw length_snoc; repnd; subst;
-  try (complete (allapply @similarity_dom; repnd; allrw; sp)).
-  rw @similarity_snoc in sim5; simpl in sim5; exrepnd; cpx; proof_irr.
-  apply equality_refl in sim2; sp.
-
-  apply @similarity_refl in sim'1; sp.
-  (* now we start using hyp2 *)
-  exrepnd.
-  lsubst_tac.
-  rw @tequality_mkc_cequiv in hyp0.
-  rw @member_eq in hyp1.
-  rw <- @member_cequiv_iff in hyp1.
-  appdup hyp0 hyp1.
-  spcast.
-
-  generalize (eqh (snoc s2a0 (z,t2) ++ s2b)); intro eqhy.
-  autodimp eqhy hyp.
-  rw @similarity_app; simpl.
-  exists (snoc s1a0 (z,t1)) s1b (snoc s2a0 (z,t2)) s2b; allrw length_snoc; sp.
-  rw @similarity_snoc; simpl.
-  exists s1a0 s2a0 t1 t2 wfsa covsa1; sp.
-
-  assert (cover_vars_upto T (csub_filter s1a0 [x]) [x])
-         as cvuT1
-         by (unfold cover_vars_upto; unfold covered in covT;
-             rw @dom_csub_csub_filter;
-             rw subvars_app_remove_nvars_r; simpl;
-             allapply @similarity_dom; repnd; allrw; sp).
-
-  generalize (simple_lsubstc_subst b x T w s1a0 p wb c6 wT cvuT1);
-    intro e; autodimp e hyp.
-  rw e in sim'2; clear e.
-
-  generalize (simple_lsubstc_subst a x T wfsa s1a0 covsa1 wa c4 wT cvuT1);
-    intro e; autodimp e hyp.
-  rw e; clear e.
-
-  apply cequivc_preserving_equality
-        with (A := substc (lsubstc b wb s1a0 c6) x
-                          (lsubstc_vars T wT (csub_filter s1a0 [x]) [x] cvuT1));
-    auto;
-    try (complete (apply cequivc_sym; eauto with cequivc)).
-
-  rw @eq_hyps_app in eqhy; exrepnd.
-  apply app_split in eqhy0; allrw length_snoc; repnd; subst; cpx;
-  try (complete (allapply @similarity_dom; repnd; allrw; sp)).
-  apply app_split in eqhy2; allrw length_snoc; repnd; subst; cpx;
-  try (complete (allapply @similarity_dom; repnd; allrw; sp)).
-
-
-  (* We're done proving the hyps_functionality part of hyp1.
-   * We now prove the similarity part of hyp1 *)
-  autodimp hyp1 hyp.
-  rw @similarity_app in sim; exrepnd; subst; cpx.
-  rw @similarity_snoc in sim5; simpl in sim5; exrepnd; subst; cpx.
-
-  generalize (hyp2 (snoc s1a0 (z,t1) ++ s1b)
-                   (snoc s2a0 (z,t1) ++ s1b)
-                   eqh); clear hyp2; intro hyp2.
-  (* before using hyp2 we have to prove a few things *)
-  autodimp hyp2 hyp.
-  rw @similarity_app; simpl.
-  exists (snoc s1a0 (z,t1)) s1b (snoc s2a0 (z,t1)) s1b; allrw length_snoc; sp.
-  rw @similarity_snoc; simpl.
-  exists s1a0 s2a0 t1 t1 w p; sp.
-
-  apply equality_refl in sim2; sp.
-
-  apply @similarity_refl in sim1; sp.
-  (* now we start using hyp2 *)
-  exrepnd.
-  lsubst_tac.
-  rw @tequality_mkc_cequiv in hyp0.
-  rw @member_eq in hyp1.
-  rw <- @member_cequiv_iff in hyp1.
-  appdup hyp0 hyp1.
-  spcast.
-
-  assert (wf_term (subst T x b))
-         as wfsb
-         by (apply @lsubst_preserves_wf_term; sp;
-             unfold wf_sub, sub_range_sat; simpl; sp; cpx; rw @nt_wf_eq; sp).
-
-  assert (cover_vars (subst T x b) s1a0)
-         as covb1 by (rw @cover_vars_eq; allapply @similarity_dom; repnd; allrw; sp).
-
-  rw @similarity_app.
-  exists (snoc s1a0 (z, t1)) s1b (snoc s2a0 (z, t2)) s2b; allrw length_snoc; sp.
-  rw @similarity_snoc; simpl.
-  exists s1a0 s2a0 t1 t2 wfsb covb1; sp.
-
-  assert (cover_vars_upto T (csub_filter s1a0 [x]) [x])
-         as cvuT1
-         by (unfold cover_vars_upto; unfold covered in covT;
-             rw @dom_csub_csub_filter;
-             rw subvars_app_remove_nvars_r; simpl;
-             allapply @similarity_dom; repnd; allrw; sp).
-
-  generalize (simple_lsubstc_subst b x T wfsb s1a0 covb1 wb c6 wT cvuT1);
-    intro e; autodimp e hyp.
-  rw e; clear e.
-
-  generalize (simple_lsubstc_subst a x T w s1a0 p wa c4 wT cvuT1);
-    intro e; autodimp e hyp.
-  rw e in sim2; clear e.
-
-  apply cequivc_preserving_equality
+  {
+    (* First, we assume that x is in the free variables of T.
+     * We can now prove that a and b depend on H only. *)
+
+    assert (covered a (vars_hyps H)) as cvah.
+    {
+      clear hyp1 hyp2.
+      allapply @vswf_hypotheses_nil_implies.
+      rw @wf_hypotheses_app in wh2; repnd.
+      rw @wf_hypotheses_snoc in wh0; repnd; allsimpl.
+      allrw @isprog_vars_eq; repnd.
+      unfold covered.
+      generalize (eqvars_free_vars_disjoint T [(x,a)]).
+      introv xx; rw @fold_subst in xx; simpl in xx.
+      apply subvars_eqvars with (s2 := vars_hyps H) in xx; auto.
+      rw subvars_prop in xx.
+      rw subvars_prop; introv j.
+      revert xx; boolvar; try (complete sp); simpl; intro xx.
+      apply xx; rw in_app_iff; rw app_nil_r; sp.
+    }
+
+    assert (covered b (vars_hyps H)) as cvbh.
+    {
+      clear hyp1 hyp2.
+      allapply @vswf_hypotheses_nil_implies.
+      rw @wf_hypotheses_app in wh1; repnd.
+      rw @wf_hypotheses_snoc in wh0; repnd; allsimpl.
+      allrw @isprog_vars_eq; repnd.
+      unfold covered.
+      pose proof (eqvars_free_vars_disjoint T [(x,b)]) as xx.
+      rw @fold_subst in xx; simpl in xx.
+      apply subvars_eqvars with (s2 := vars_hyps H) in xx; auto.
+      rw subvars_prop in xx.
+      rw subvars_prop; introv j.
+      revert xx; boolvar; try (complete sp); simpl; intro xx.
+      apply xx; rw in_app_iff; rw app_nil_r; sp.
+    }
+
+    assert (covered T (snoc (vars_hyps H) x)) as covT.
+    {
+      clear hyp1 hyp2.
+      allapply @vswf_hypotheses_nil_implies.
+      rw @wf_hypotheses_app in wh1; repnd.
+      rw @wf_hypotheses_snoc in wh0; repnd; allsimpl.
+      allrw @isprog_vars_eq; repnd.
+      unfold covered.
+      pose proof (eqvars_free_vars_disjoint T [(x,b)]) as xx.
+      rw @fold_subst in xx; simpl in xx.
+      apply subvars_eqvars with (s2 := vars_hyps H) in xx; auto.
+      rw subvars_prop in xx.
+      rw subvars_prop; introv j.
+      revert xx; boolvar; try (complete sp); simpl; intro xx.
+      rw in_snoc.
+      destruct (deq_nvar x0 x); subst; sp.
+      left; apply xx; rw in_app_iff; rw app_nil_r; rw in_remove_nvars; rw in_single_iff; sp.
+    }
+
+    assert (!LIn z (free_vars a))
+      as niza
+        by (intro j; unfold covered in cvah;
+            rw subvars_prop in cvah; apply cvah in j; sp).
+
+    assert (!LIn z (free_vars b))
+      as nizb
+        by (intro j; unfold covered in cvbh;
+            rw subvars_prop in cvbh; apply cvbh in j; sp).
+
+    assert (disjoint (free_vars a) (vars_hyps J))
+      as daj
+        by (introv j k; unfold covered in cvah;
+            rw subvars_prop in cvah; apply cvah in j; sp;
+            apply disjHJ in j; sp).
+
+    assert (disjoint (free_vars b) (vars_hyps J))
+      as dbj
+        by (introv j k; unfold covered in cvbh;
+            rw subvars_prop in cvbh; apply cvbh in j; sp;
+            apply disjHJ in j; sp).
+
+    assert (subvars (free_vars (subst T x a)) (vars_hyps H)) as svaH.
+    {
+      pose proof (eqvars_free_vars_disjoint T [(x,a)]) as xx.
+      apply eqvars_sym in xx.
+      apply subvars_eqvars with (s2 := vars_hyps H) in xx; auto.
+      rw subvars_prop; introv; simpl.
+      rw in_app_iff; rw in_remove_nvars; rw in_single_iff.
+      boolvar; simpl; try (complete sp).
+      rw app_nil_r; intro j; repdors; repnd.
+      try (complete (unfold covered in covT; rw subvars_prop in covT;
+                     apply covT in j1; rw in_snoc in j1; allrw; sp)).
+      try (complete (unfold covered in cvah; rw subvars_prop in cvah;
+                     apply cvah in j; sp)).
+    }
+
+    assert (subvars (free_vars (subst T x b)) (vars_hyps H)) as svbH.
+    {
+      pose proof (eqvars_free_vars_disjoint T [(x,b)]) as xx.
+      apply eqvars_sym in xx.
+      apply subvars_eqvars with (s2 := vars_hyps H) in xx; auto.
+      rw subvars_prop; introv; simpl.
+      rw in_app_iff; rw in_remove_nvars; rw in_single_iff.
+      boolvar; simpl; try (complete sp).
+      rw app_nil_r; intro j; repdors; repnd.
+      try (complete (unfold covered in covT; rw subvars_prop in covT;
+                     apply covT in j1; rw in_snoc in j1; allrw; sp)).
+      try (complete (unfold covered in cvbh; rw subvars_prop in cvbh;
+                     apply cvbh in j; sp)).
+    }
+
+    assert (subvars (free_vars T) (x :: vars_hyps H))
+      as svTH
+        by (rw subvars_prop in covT; rw subvars_prop; introv j;
+            apply covT in j; rw in_snoc in j; simpl; sp).
+
+    generalize (hyp1 s1 s2); clear hyp1; intro hyp1.
+
+    autodimp hyp1 hyp.
+
+    {
+      (* First, we prove that the hypotheses of the first sequent are functional *)
+      introv sim'.
+      rw @similarity_app in sim'; simpl in sim'; exrepnd; subst; allrw length_snoc; cpx.
+      rw @similarity_snoc in sim'5; simpl in sim'5; exrepnd; subst; allrw length_snoc; cpx.
+
+      rw @eq_hyps_app.
+      exists (snoc s1a0 (z, t1)) s1b (snoc s2a0 (z, t2)) s2b.
+      allrw length_snoc; dands; try (complete sp).
+
+      {
+        assert (cover_vars (subst T x b) s2a0)
+          as cov2
+            by (apply cover_vars_change_sub with (sub1 := s1a0); sp;
+                allapply @similarity_dom; repnd; allrw; sp).
+
+        rw @eq_hyps_snoc; simpl.
+        exists s1a0 s2a0 t1 t2 w p cov2.
+        dands; try (complete sp).
+
+        {
+          assert (wf_term (subst T x a))
+            as wfsa
+              by (apply @lsubst_preserves_wf_term; simpl;
+                  unfold wf_sub, sub_range_sat; simpl; sp; cpx; rw @nt_wf_eq; sp).
+
+          assert (cover_vars (subst T x a) s1a0)
+            as cova1 by (rw @cover_vars_eq; allapply @similarity_dom; repnd; allrw; sp).
+
+          dup eqh as hf.
+
+          apply hyps_functionality_init_seg
+            with (s3 := s2b) in eqh; auto.
+          apply @hyps_functionality_init_seg_snoc2
+            with (t' := t2) (w := wfsa) (c := cova1) in eqh.
+          apply eqh in sim'6; auto.
+
+          generalize (hyp2 (snoc s1a0 (z,t1) ++ s1b) s2 hf sim); clear hyp2; intro hyp2; exrepnd.
+          lsubst_tac.
+          apply equality_in_mkc_cequiv in hyp1; repnd.
+          clear hyp2 hyp3.
+          spcast.
+
+          assert (cover_vars_upto T (csub_filter s1a0 [x]) [x])
+            as covT1
+              by (unfold cover_vars_upto; unfold covered in covT;
+                  rw @dom_csub_csub_filter;
+                  rw subvars_app_remove_nvars_r; simpl;
+                  allapply @similarity_dom; repnd; allrw; sp).
+
+          generalize (simple_lsubstc_subst b x T w s1a0 p wb c6 wT covT1);
+            introv xx; autodimp xx hyp.
+          rw xx in sim'2; clear xx.
+
+          generalize (simple_lsubstc_subst a x T wfsa s1a0 cova1 wa c4 wT covT1);
+            introv xx; autodimp xx hyp.
+          rw xx; clear xx.
+
+          apply cequivc_preserving_equality
+            with (A := substc (lsubstc b wb s1a0 c6) x
+                              (lsubstc_vars T wT (csub_filter s1a0 [x]) [x] covT1));
+            auto;
+            try (complete (apply cequivc_sym; eauto with cequivc)).
+        }
+
+        {
+          (* now we prove the tequality of T[x\b] *)
+          assert (wf_term (subst T x a))
+            as wfsa
+              by (apply @lsubst_preserves_wf_term; sp;
+                  unfold wf_sub, sub_range_sat; simpl; sp; cpx; rw @nt_wf_eq; sp).
+
+          assert (cover_vars (subst T x a) s1a0)
+            as covsa1 by (rw @cover_vars_eq; allapply @similarity_dom; repnd; allrw; sp).
+
+          generalize (eqh (snoc s2a0 (z,t1) ++ s1b)); intro eqhy.
+          autodimp eqhy hyp.
+          rw @similarity_app; simpl.
+          exists (snoc s1a0 (z, t1)) s1b (snoc s2a0 (z, t1)) s1b; allrw length_snoc; sp.
+          rw @similarity_snoc; simpl.
+          exists s1a0 s2a0 t1 t1 wfsa covsa1; sp.
+
+          {
+            rw @similarity_app in sim; simpl in sim; exrepnd.
+            apply app_split in sim0; allrw length_snoc; repnd; subst;
+              try (complete (allapply @similarity_dom; repnd; allrw; sp)).
+            rw @similarity_snoc in sim5; simpl in sim5; exrepnd; cpx; proof_irr.
+            apply equality_refl in sim2; sp.
+          }
+
+          {
+            apply @similarity_refl in sim'1; sp.
+          }
+
+          {
+            rw @eq_hyps_app in eqhy; simpl in eqhy; exrepnd.
+            apply app_split in eqhy0; allrw length_snoc; repnd; subst; cpx;
+              try (complete (allapply @similarity_dom; repnd; allrw; sp)).
+            apply app_split in eqhy2; allrw length_snoc; repnd; subst; cpx;
+              try (complete (allapply @similarity_dom; repnd; allrw; sp)).
+            rw @eq_hyps_snoc in eqhy5; simpl in eqhy5; exrepnd; cpx.
+
+            (* now we prove the tequality from eqhy0 *)
+
+            generalize (hyp2 (snoc s1a (z,t0) ++ s2b0)
+                             (snoc s2a (z,t0) ++ s2b0)
+                             eqh); clear hyp2; intro hyp2.
+            (* before using hyp2 we have to prove a few things *)
+            autodimp hyp2 hyp.
+
+            {
+              rw @similarity_app; simpl.
+              exists (snoc s1a (z,t0)) s2b0 (snoc s2a (z,t0)) s2b0; allrw length_snoc; sp.
+              rw @similarity_snoc; simpl.
+              exists s1a s2a t0 t0 w0 p1; sp.
+
+              {
+                rw @similarity_app in sim; simpl in sim; exrepnd.
+                apply app_split in sim0; allrw length_snoc; repnd; subst;
+                  try (complete (allapply @similarity_dom; repnd; allrw; sp)).
+                rw @similarity_snoc in sim5; simpl in sim5; exrepnd; cpx; proof_irr.
+                apply equality_refl in sim2; sp.
+              }
+
+              {
+                apply @similarity_refl in sim'1; sp.
+              }
+            }
+
+            (* now we start using hyp2 *)
+            exrepnd.
+            lsubst_tac.
+            rw @tequality_mkc_cequiv in hyp0.
+            apply equality_in_mkc_cequiv in hyp1; repnd.
+            clear hyp2 hyp3.
+            appdup hyp0 hyp1.
+            spcast.
+
+            assert (cover_vars_upto T (csub_filter s1a [x]) [x])
+              as cvuT1
+                by (unfold cover_vars_upto; unfold covered in covT;
+                    rw @dom_csub_csub_filter;
+                    rw subvars_app_remove_nvars_r; simpl;
+                    allapply @similarity_dom; repnd; allrw; sp).
+
+            assert (cover_vars_upto T (csub_filter s2a [x]) [x])
+              as cvuT2
+                by (unfold cover_vars_upto; unfold covered in covT;
+                    rw @dom_csub_csub_filter;
+                    rw subvars_app_remove_nvars_r; simpl;
+                    allapply @similarity_dom; repnd; allrw; sp).
+
+            generalize (simple_lsubstc_subst b x T w s1a p wb c6 wT cvuT1);
+              intro xx; autodimp xx hyp.
+            rw xx; clear xx.
+
+            generalize (simple_lsubstc_subst b x T w s2a cov2 wb c10 wT cvuT2);
+              intro xx; autodimp xx hyp.
+            rw xx; clear xx.
+
+            generalize (simple_lsubstc_subst a x T w0 s1a p1 wa c4 wT cvuT1);
+              intro xx; autodimp xx hyp.
+            rw xx in eqhy0; clear xx.
+
+            generalize (simple_lsubstc_subst a x T w0 s2a p2 wa c8 wT cvuT2);
+              intro xx; autodimp xx hyp.
+            rw xx in eqhy0; clear xx.
+
+            apply tequality_respects_cequivc_left
+              with (T1 := substc (lsubstc a wa s1a c4) x
+                                 (lsubstc_vars T wT (csub_filter s1a [x]) [x] cvuT1));
+              try (complete (eauto with cequivc)).
+
+            apply tequality_respects_cequivc_right
+              with (T2 := substc (lsubstc a wa s2a c8) x
+                                 (lsubstc_vars T wT (csub_filter s2a [x]) [x] cvuT2));
+              auto;
+              try (complete (eauto with cequivc)).
+          }
+        }
+      }
+
+
+      (* Now we prove the sub_eq_hyps *)
+
+      assert (wf_term (subst T x a))
+        as wfsa
+          by (apply @lsubst_preserves_wf_term; sp;
+              unfold wf_sub, sub_range_sat; simpl; sp; cpx; rw @nt_wf_eq; sp).
+
+      assert (cover_vars (subst T x a) s1a0)
+        as covsa1 by (rw @cover_vars_eq; allapply @similarity_dom; repnd; allrw; sp).
+
+      generalize (hyp2 (snoc s1a0 (z,t1) ++ s1b)
+                       (snoc s2a0 (z,t1) ++ s1b)
+                       eqh); clear hyp2; intro hyp2.
+      (* before using hyp2 we have to prove a few things *)
+      autodimp hyp2 hyp.
+
+      {
+        rw @similarity_app; simpl.
+        exists (snoc s1a0 (z,t1)) s1b (snoc s2a0 (z,t1)) s1b; allrw length_snoc; sp.
+
+        {
+          rw @similarity_snoc; simpl.
+          exists s1a0 s2a0 t1 t1 wfsa covsa1; sp.
+
+          rw @similarity_app in sim; simpl in sim; exrepnd.
+          apply app_split in sim0; allrw length_snoc; repnd; subst;
+            try (complete (allapply @similarity_dom; repnd; allrw; sp)).
+          rw @similarity_snoc in sim5; simpl in sim5; exrepnd; cpx; proof_irr.
+          apply equality_refl in sim2; sp.
+        }
+
+        apply @similarity_refl in sim'1; sp.
+      }
+
+      (* now we start using hyp2 *)
+      exrepnd.
+      lsubst_tac.
+      rw @tequality_mkc_cequiv in hyp0.
+      apply equality_in_mkc_cequiv in hyp1; repnd.
+      clear hyp2 hyp3.
+      appdup hyp0 hyp1.
+      spcast.
+
+      generalize (eqh (snoc s2a0 (z,t2) ++ s2b)); intro eqhy.
+      autodimp eqhy hyp.
+      rw @similarity_app; simpl.
+      exists (snoc s1a0 (z,t1)) s1b (snoc s2a0 (z,t2)) s2b; allrw length_snoc; sp.
+
+      {
+        rw @similarity_snoc; simpl.
+        exists s1a0 s2a0 t1 t2 wfsa covsa1; sp.
+
+        assert (cover_vars_upto T (csub_filter s1a0 [x]) [x])
+          as cvuT1
+            by (unfold cover_vars_upto; unfold covered in covT;
+                rw @dom_csub_csub_filter;
+                rw subvars_app_remove_nvars_r; simpl;
+                allapply @similarity_dom; repnd; allrw; sp).
+
+        generalize (simple_lsubstc_subst b x T w s1a0 p wb c6 wT cvuT1);
+          intro xx; autodimp xx hyp.
+        rw xx in sim'2; clear xx.
+
+        generalize (simple_lsubstc_subst a x T wfsa s1a0 covsa1 wa c4 wT cvuT1);
+          intro xx; autodimp xx hyp.
+        rw xx; clear xx.
+
+        apply cequivc_preserving_equality
+          with (A := substc (lsubstc b wb s1a0 c6) x
+                            (lsubstc_vars T wT (csub_filter s1a0 [x]) [x] cvuT1));
+          auto;
+          try (complete (apply cequivc_sym; eauto with cequivc)).
+      }
+
+      rw @eq_hyps_app in eqhy; exrepnd.
+      apply app_split in eqhy0; allrw length_snoc; repnd; subst; cpx;
+        try (complete (allapply @similarity_dom; repnd; allrw; sp)).
+      apply app_split in eqhy2; allrw length_snoc; repnd; subst; cpx;
+        try (complete (allapply @similarity_dom; repnd; allrw; sp)).
+    }
+
+
+    (* We're done proving the hyps_functionality part of hyp1.
+     * We now prove the similarity part of hyp1 *)
+    autodimp hyp1 hyp.
+
+    {
+      rw @similarity_app in sim; exrepnd; subst; cpx.
+      rw @similarity_snoc in sim5; simpl in sim5; exrepnd; subst; cpx.
+
+      generalize (hyp2 (snoc s1a0 (z,t1) ++ s1b)
+                       (snoc s2a0 (z,t1) ++ s1b)
+                       eqh); clear hyp2; intro hyp2.
+      (* before using hyp2 we have to prove a few things *)
+      autodimp hyp2 hyp.
+
+      {
+        rw @similarity_app; simpl.
+        exists (snoc s1a0 (z,t1)) s1b (snoc s2a0 (z,t1)) s1b; allrw length_snoc; sp.
+
+        {
+          rw @similarity_snoc; simpl.
+          exists s1a0 s2a0 t1 t1 w p; sp.
+
+          apply equality_refl in sim2; sp.
+        }
+
+        apply @similarity_refl in sim1; sp.
+      }
+
+      (* now we start using hyp2 *)
+      exrepnd.
+      lsubst_tac.
+      rw @tequality_mkc_cequiv in hyp0.
+      apply equality_in_mkc_cequiv in hyp1; repnd.
+      clear hyp2 hyp3.
+      appdup hyp0 hyp1.
+      spcast.
+
+      assert (wf_term (subst T x b))
+        as wfsb
+          by (apply @lsubst_preserves_wf_term; sp;
+              unfold wf_sub, sub_range_sat; simpl; sp; cpx; rw @nt_wf_eq; sp).
+
+      assert (cover_vars (subst T x b) s1a0)
+        as covb1 by (rw @cover_vars_eq; allapply @similarity_dom; repnd; allrw; sp).
+
+      rw @similarity_app.
+      exists (snoc s1a0 (z, t1)) s1b (snoc s2a0 (z, t2)) s2b; allrw length_snoc; sp.
+      rw @similarity_snoc; simpl.
+      exists s1a0 s2a0 t1 t2 wfsb covb1; sp.
+
+      assert (cover_vars_upto T (csub_filter s1a0 [x]) [x])
+        as cvuT1
+          by (unfold cover_vars_upto; unfold covered in covT;
+              rw @dom_csub_csub_filter;
+              rw subvars_app_remove_nvars_r; simpl;
+              allapply @similarity_dom; repnd; allrw; sp).
+
+      generalize (simple_lsubstc_subst b x T wfsb s1a0 covb1 wb c6 wT cvuT1);
+        intro xx; autodimp xx hyp.
+      rw xx; clear xx.
+
+      generalize (simple_lsubstc_subst a x T w s1a0 p wa c4 wT cvuT1);
+        intro xx; autodimp xx hyp.
+      rw xx in sim2; clear xx.
+
+      apply cequivc_preserving_equality
         with (A := substc (lsubstc a wa s1a0 c4) x
                           (lsubstc_vars T wT (csub_filter s1a0 [x]) [x] cvuT1));
-    auto;
-    try (complete (eauto with cequivc)).
+        auto;
+        try (complete (eauto with cequivc)).
+    }
 
 
-  (* now we use hyp1 *)
-  exrepnd; proof_irr; GC; sp.
+    (* now we use hyp1 *)
+    exrepnd; proof_irr; GC; sp.
+  }
 
 
 
   (* now we're done to the case where x is not in the free_vars of t *)
   assert (subst T x a = T)
-         as e1 by (apply @lsubst_trivial3; introv j; rw in_single_iff in j; cpx).
+    as e1 by (apply @lsubst_trivial3; introv j; rw in_single_iff in j; cpx).
   allrw e1; clear e1.
   assert (subst T x b = T)
-         as e2 by (apply @lsubst_trivial3; introv j; rw in_single_iff in j; cpx).
+    as e2 by (apply @lsubst_trivial3; introv j; rw in_single_iff in j; cpx).
   allrw e2; clear e2.
 
   generalize (hyp1 s1 s2 eqh sim); clear hyp1; intro hyp1; exrepnd; proof_irr; sp.
